rt spec+proof: prove preemptionPoint_ccorres
This also adjusts the ASpec and Haskell definitions of
preemption_point/preemptionPoint to more closely align with the C.

Signed-off-by: Michael McInerney <michael.mcinerney@proofcraft.systems>

spec/haskell/src/SEL4/Model/StateData.lhs
@@ -516,3 +516,8 @@ An assert that will say that the idle thread is not in a ready queue
 
 > idleThreadNotQueued :: KernelState -> Bool
 > idleThreadNotQueued _ = True
+
+An assert that will say that there is a scheduling context at the given pointer
+
+> sc_at'_asrt :: PPtr SchedContext -> KernelState -> Bool
+> sc_at'_asrt _ _ = True
