spec/abstract/KHeap_A.thy
@@ -650,21 +650,19 @@ where
                              else modify (\<lambda>s. s\<lparr> domain_time := domain_time - consumed \<rparr>)
   od"
 
-definition
-  preemption_point :: "(unit,'z::state_ext) p_monad"
-where
+definition preemption_point :: "(unit,'z::state_ext) p_monad" where
   "preemption_point \<equiv> doE
      liftE $ do_extended_op update_work_units;
      OR_choiceE work_units_limit_reached
      (doE liftE $ do_extended_op reset_work_units;
           liftE $ update_time_stamp;
           irq_opt \<leftarrow> liftE $ do_machine_op (getActiveIRQ True);
+          exp \<leftarrow> liftE $ gets is_cur_domain_expired;
           cur_sc \<leftarrow> liftE $ gets cur_sc;
           consumed \<leftarrow> liftE $ gets consumed_time;
-          test \<leftarrow> liftE $ andM (get_sc_active cur_sc)
-                               (get_sc_refill_sufficient cur_sc consumed);
-          exp \<leftarrow> liftE $ gets is_cur_domain_expired;
-          whenE (\<not>test \<or> exp \<or> irq_opt \<noteq> None) $ throwError ()
+          active \<leftarrow> liftE $ get_sc_active cur_sc;
+          sufficient \<leftarrow> liftE $ gets $ read_sc_refill_sufficient cur_sc consumed;
+          whenE ((irq_opt \<noteq> None) \<or> exp \<or> \<not> (active \<and> sufficient = Some True)) (throwError ())
       odE)
      (returnOk ())
    odE"
